\documentclass[12pt,letterpaper,titlepage]{article}

\usepackage{fontspec}
\defaultfontfeatures{Mapping=tex-text}
\usepackage{xunicode}
\usepackage{xltxtra}
\usepackage{amsmath}
\usepackage{pdfpages}
\usepackage{mathtools}
\usepackage{amsfonts}
\usepackage{amssymb}
\setcounter{secnumdepth}{0}
\usepackage{nameref}
\usepackage{enumitem}
\usepackage{environ}

\showboxdepth=\maxdimen
\showboxbreadth=\maxdimen

\usepackage[tocflat]{tocstyle}
\usetocstyle{allwithdot}
\usepackage[bottom]{footmisc}

\usepackage{paracol}
\usepackage{wrapfig}
\globalcounter{table}
\globalcounter{figure}
\usepackage{graphicx}
\usepackage[left=1in,right=1in,top=1in,bottom=1in]{geometry}
\graphicspath{{img/}}

\author{Jacob Abel}
\title{	Homework 7
	\\\large MATH2534 CRN:15708
}

\setlength{\parskip}{0.5em}

\begin{document}
\maketitle
\begin{raggedright}
Prove the following statements using strong mathematical induction.

\begin{enumerate}

\item Let $a \neq b$ be two distinct integers, and let $n \geq 1$ be any integer. Prove that $a^n - b^n$ is divisible by $a - b$.

Let $\forall a, b, n \in \mathbb{Z}, a\neq b, n \geq 1$.

$P(1):\;a^1-b^1 = a-b \implies (a-b)|(a^1-b^1)$

$P(2):\;a^2-b^2 = (a-b)(a+b) \implies (a-b)|(a^2-b^2)$

$P(3):\;a^3-b^3 = (a-b)(a+b)(a^2-b^2) \implies (a-b)|(a^3-b^3)$

Suppose this holds true for $P(n):\;(a-b)|(a^n-b^n)$.

$P(n+1):\;(a-b)|(a^{n+1}-b^{n+1})$

$a^{n+1}-b^{n+1} = a\times a^n - b\times b^n =aa^n-ab^n+ab^n-bb^n=(a^n-b^n)a+(a-b)b^n$

$a^n-b^n$ and $a-b$ are both divisible by $a-b$. This means that $a^{n+1}-b^{n+1}$ is divisible by $a-b$.

Therefore by induction, $a^n-b^n$ is divisible by $a-b$ for all $n \geq 1$.

\item Let $a_1, a_2, a_3, ...$ be a sequence such that $a_1 = 1, a_2 = 1$ and $a_k = 2a_{k−1} + 3a_{k−2}$ for $k \geq 3$. Prove that $a_n \leq 2 \times 3^{n−2}$ for all $n \geq 3$.

Let $\forall k, n, \exists a \in \mathbb{Z}, n \geq 3, k \geq 3, a_k = 2a_{k−1} + 3a_{k−2}$.

$P(1):\; a_1 = 1 \leq 2\times 3^{1-2} = \frac{2}{3}$

$P(2):\; a_2 = 1 \leq 2\times 3^{2-2} = 2$

$P(3):\; a_3 = 2a_{3-1} + 3a_{3-2} = 2a_2 + 3a_1 = 2+3 = 5 \leq 2\times 3^{3-2} = 6 \implies 5 \leq 6$

Suppose this holds true for $P(n):\;a_n \leq 2 \times 3^{n−2}$.

$P(n+1):\;a_{n+1} \leq 2 \times 3^{n + 1 −2}$

$a_{n+1} = 2a_{n+1−1} + 3a_{n+1−2} = 2a_n + 3a_{n−1}$

$ 2 \times 3^{n + 1 −2} = 2\times 3^{n-1}$

$2a_n + 3a_{n−1} \leq 2\times 3^{n-1}$

As $a_n \leq 2\times 3^{n-2}$, $a_{n-1} \leq 2\times 3^{n-3}$

$2a_n + 3a_{n−1} \leq 2\times2\times 3^{n-2} + 3\times2\times 3^{n-3} = 4\times 3^{n-2} + 2\times 3^{n-2}=6\times 3^{n-2}=2\times 3^{n-1}$

$2\times 3^{n-1} \leq 2\times 3^{n-1}$

Therefore by induction, $a_n \leq 2 \times 3^{n−2}$ for all $n\geq 3$.

\clearpage
\item Let $a_1, a_2, a_3, ...$ be a sequence such that $a_1 = 1, a_2 = 8$ and $a_k = a_{k−1} + 2a_{k−2}$ for $k \geq 3$. Prove that $a_n = 3 \times 2^{n−1} + 2(−1)^n$ for all $n \geq 1$.

Let $\forall k, n, \exists a \in \mathbb{Z}, n \geq 1, k \geq 3, a_k = a_{k−1} + 2a_{k−2}$.

$P(1):\; a_1 = 1 = 3 \times 2^{1−1} + 2(−1)^1=3-2=1$

$P(2):\; a_2 = 8 = 3 \times 2^{2−1} + 2(−1)^2=6+2=8$

$P(3):\; a_3 = a_{3−1} + 2a_{3−2} = a_2 + 2a_1 = 8 + 2 = 10 = 3 \times 2^{3−1} + 2(−1)^3 = 12 - 2 = 10$

Suppose this holds true for $P(n):\; a_n = 3 \times 2^{n−1} + 2(−1)^n$.

$P(n+1):\; a_{n+1} = 3 \times 2^{n+1−1} + 2(−1)^{n-1} = 3 \times 2^{n} - 2(−1)^{n}$

$a_{n+1} = a_{n+1−1} + 2a_{n+1-2} = a_{n} + 2a_{n-1}$

As $a_n = 3 \times 2^{n−1} + 2(−1)^n$, $a_{n-1} = 3 \times 2^{n−2} + 2(−1)^{n-1}$

$a_{n+1} = (3 \times 2^{n−1} + 2(−1)^n) + 2(3 \times 2^{n−2} + 2(−1)^{n-1}) = 3 \times 2^{n} - 2(−1)^n$

$a_{n+1} = 3 \times 2^{n} - 2(−1)^n = 3 \times 2^{n} - 2(−1)^n$

Therefore by induction, $P(n):\; a_n = 3 \times 2^{n−1} + 2(−1)^n$ for all $n\geq 1$

\item Let $a_1, a_2, a_3, ...$ be a sequence such that $a_1 = 1, a_2 = 1, a_3 = 3$ and $a_k = a_{k−1} + a_{k−2} + a_{k−3}$ for $k \geq 4$. Prove that $a_n < 2^n$ for all $n \geq 1$.

Let $\forall k, n, \exists a \in \mathbb{Z}, n \geq 1, k \geq 4, a_k = a_{k−1} + a_{k−2} + a_{k−3}$.

$P(1):\; a_1 = 1 < 2^1 = 2$

$P(2):\; a_2 = 1 < 2^2 = 4$

$P(3):\; a_3 = 3 < 2^3 = 8$

$P(4):\; a_4 = a_{4−1} + a_{4−2} + a_{4−3} = 8 + 4 + 2 = 14 < 2^4 = 16$

Suppose this holds true for $P(n):\; a_n < 2^n$.

$P(n+1):\; a_{n+1} < 2^{n+1}$

$a_{n+1} = a_{n+1−1} + a_{n+1−2} + a_{n+1−3} = a_n + a_{n−1} + a_{n−2}$

As $a_n < 2^n$, $a_{n-1} < 2^{n-1}$ and $a_{n-2} < 2^{n-2}$

$a_{n+1} < 2^n + 2^{n-1} + 2^{n-2} = \frac{7}{4}2^n = 7\times 2^{n-2} < 2^{n+1}$

$7\times 2^{n-2} < 2^{n+1}$

Therefore by induction, $P(n):\; a_n < 2^n$ for all $n \geq 1$.

\clearpage
\item Prove that every amount of postage that is at least 44\textcent{} can be made from 5\textcent{} and 12\textcent{} stamps.

Let $\forall n, \exists x, y \in \mathbb{Z}, n \geq 44$.

$P(44):\; 44 = 5\times 4 + 12\times 2$

$P(45):\; 45 = 5\times 9 + 12\times 0$

$P(46):\; 46 = 5\times 2 + 12\times 3$

$P(47):\; 47 = 5\times 7 + 12\times 1$

$P(48):\; 48 = 5\times 0 + 12\times 4$

Suppose this holds true for $P(n):\; n = 5x + 12y$.

$P(n+1):\; n+1 = 5x + 12y$

Because we can have shown that 48\textcent{} postage can be made from 5\textcent{} and 12\textcent{} stamps, we can assume that $n+1\geq 49$

$44\leq (n+1) - 5 \leq n\implies 44 \leq n-4\implies 15\leq n$

$(n+1)-5=5x+12y\implies n+1 = 5(x+1)+12y$

$n+1 = 5(x+1)+12y, x+1 > 0, y \geq 0$

Therefore by induction, every amount of postage that is at least 44\textcent{} can be made from 5\textcent{} and 12\textcent{} stamps.

\end{enumerate}
\end{raggedright}
\end{document}
